Day01 in 2022 in coq

2022/coq/Day01.v
@@ -5,50 +5,28 @@ From Coq Require Extraction.
 
 Require Import Coq.Arith.PeanoNat.
 Require Import Coq.Numbers.DecimalString.
+Require Import Coq.Sorting.Mergesort.
+Require Import Coq.Sorting.Sorting.
+Require Import Coq.Structures.Orders.
 
 Require Import Parsec.Core.
 
 Require Import ExtLib.Data.Option.
-
-(*
-Print Visibility.
-
-Definition istchar (a : ascii) : bool :=
-  isalpha a ||| isdigit a ||| in_string "!#$%&'*+-.^_`|~" a.
-
-Definition parseToken : parser string :=
-  string_of_list_ascii <$> many1 (satisfy istchar).
-
-Goal parse parseToken "GET / HTTP/1.1" = inr ("GET", " / HTTP/1.1").
-Proof. reflexivity. Qed.
-*)
-
-Example parseDecExample : parse parseDec "123" = inr (123%N, "").
-Proof. unfold parse. simpl. reflexivity. Qed.
-
-
-Example parseDecExample2 : parse parseDec "123
-" = inr (123%N, "
-").
-Proof. unfold parse. simpl. reflexivity. Qed.
-
-Example parseLFExample : parse parseLF "
-" = inr ("010"%char, "").
-Proof. unfold parse. simpl. reflexivity. Qed.
-
 
 Definition singleNumParser : parser N :=
   n <- parseDec ;;
   parseLF ;;
   pure n.
 
+Print singleNumParser.
+
 Example singleNumParserExample : parse singleNumParser "123
 " = inr (123%N, "").
 Proof. unfold parse. simpl. reflexivity. Qed.
 
-Definition numsParser : parser (list N) := many1 singleNumParser.
+Definition elfNumsParser : parser (list N) := many1 singleNumParser.
 
-Example numsParserExample : parse numsParser "199
+Example elfNumsParserExample : parse elfNumsParser "199
 200
 208
 210
@@ -56,174 +34,99 @@ Example numsParserExample : parse numsParser "199
 " = inr ([199%N; 200%N; 208%N; 210%N; 200%N], "").
 Proof. unfold parse. simpl. reflexivity. Qed.
 
-Definition parseInput (str : string): option (list N) :=
-  match parse numsParser str with
+
+
+Definition many_' {T : Type} (acc : list T) (fuel : nat) (p : @parser string T) :
+    @parser string (list T) :=
+  match fuel with
+  | O => pure []
+  | S fuel' => pure []
+  end.
+
+Definition sepBy1 {P} {T} {SEP} (p : parser T)
+    (s : @parser P SEP) : @parser P (list T) :=
+  x <- p ;;
+  xs <- many (s ;; p);;
+  pure (x :: xs). 
+
+Definition elvesParser : parser (list (list N)) :=
+  sepBy1 elfNumsParser parseLF.
+
+Example elvesParserExample : parse elvesParser "199
+200
+208
+
+10000
+
+5000
+6000
+" = inr ([[199%N; 200%N; 208%N]; [10000%N]; [5000%N; 6000%N]], "").
+Proof. auto. Qed.
+
+
+Definition parseInput (str : string): option (list (list N)) :=
+  match parse elvesParser str with
   | inr (res, "") => Some res
   | _ => None
   end.
   
-Example parseInputExample : parseInput "199
-200
-208
-210
-200
-" = Some [199%N; 200%N; 208%N; 210%N; 200%N].
-Proof. unfold parseInput. unfold parse. simpl. reflexivity. Qed.
+Example parseInputExample : parseInput "1000
+2000
+3000
 
-Print N.
+4000
 
-Print positive.
+5000
+6000
 
-Compute (xI xH).
+7000
+8000
+9000
 
-Definition n_to_string (n : N): string := NilEmpty.string_of_uint (N.to_uint n).
+10000
+" = Some [[1000%N;2000%N;3000%N];[4000%N];[5000%N; 6000%N];[7000%N; 8000%N; 9000%N];[10000%N]].
+Proof. auto. Qed.
 
-Compute (n_to_string 100).
+Definition n_to_string (n : N): string :=
+  NilEmpty.string_of_uint (N.to_uint n).
 
-Local Open Scope N_scope.
+Local Open Scope N_scope.  
 
-Fixpoint count_increases (l : list N): N :=
-  match l with
-  | h1 :: t =>
-      match t with
-      | h2 :: t2 =>
-          (if 1 <=? N.sub h2 h1 then 1 else 0) + count_increases t
-      | [] => 0
-      end
-  | _ => 0
-  end.
+Definition sum_elf (l : list N): N := fold_right Nplus N0 l.
 
 Example count_increases_example :
-  count_increases [199%N; 200%N; 208%N; 210%N; 200%N; 207%N; 240%N; 269%N; 260%N; 263%N] = 7.
+  sum_elf [7000%N; 8000%N; 9000%N] = 24000%N.
 Proof. reflexivity. Qed.
 
-Inductive count_increases_relation : (list N) -> N -> Prop :=
-  | Count_Increases_EmptyList : count_increases_relation [] 0
-  | Count_Increases_SingleItem (x : N) : count_increases_relation [x] 0
-  | Count_Increases_LT (x y amt : N) (rest : list N) :
-      x < y ->
-      count_increases_relation (y :: rest) amt ->
-      count_increases_relation (x :: y :: rest) (1 + amt)
-  | Count_Increases_NLT (x y amt : N) (rest : list N) :
-      x >= y ->
-      count_increases_relation (y :: rest) amt ->
-      count_increases_relation (x :: y :: rest) amt
-  .
-  
-Lemma gt_1_implies_lt : forall (x y : N), 1 <= x - y -> y < x.
-Proof.
-  (* unfold N.lt. unfold N.le. unfold not.*) (* unfold N.compare. *)
-  intros x y.
-  destruct (1 ?= x - y) eqn:E.
-  + apply N.compare_eq in E.
-    symmetry in E.
-    assert (1 <> 0).
-    { intros H. discriminate H. }
-    set (G := N.add_sub_eq_nz x y 1 H E).
-    rewrite <- G.
-    intros.
-    apply N.lt_add_pos_r. reflexivity.
-  + intros H.
-    clear E.
-    Check N.le_add_le_sub_r.
-    induction y using N.peano_rect.
-    - simpl in H.
-      unfold N.lt.
-       (* unfold N.le in H.
-    (* rewrite <- (N.le_add_le_sub_r 1 x y) in H. *)
-    set (G :=N.le_add_le_sub_r 1 x y). *)
-    Admitted.
-  
-Theorem count_increases_relation_true :
-  forall l amt, count_increases l = amt <-> count_increases_relation l amt.
-Proof.
-  split.
-  - destruct l as [ | h1 [ | h2 rest ] ].
-    + simpl. intros H. subst amt. constructor.
-    + simpl. intros H. subst amt. constructor.
-    + simpl. 
-      set (G := N.leb_spec0 1%N (h2 - h1)).
-      inversion G.
-      * intros H1.
-        subst amt.
-        apply Count_Increases_LT.
-        symm
-        Admitted.
-    
+Definition find_most_elf (elves : list (list N)): N :=
+  fold_right N.max 0 (map sum_elf elves).
 
-Theorem count_increases_adds_one_for_increase :
-  forall x y rest, x < y -> 1 + count_increases (y :: rest) = count_increases (x :: y :: rest).
-Proof.
-  intros x y rest H.
-  unfold count_increases at 2.
-  set (G := N.leb_spec0 1%N (y - x)).
-  inversion G.
-  - reflexivity.
-  - fold count_increases.
-    clear G H1.
-    exfalso.
-    symmetry in H0.
-    apply N.leb_gt in H0.
-    apply N.lt_1_r in H0.
-    apply N.sub_gt in H.
-    apply H. assumption.
+Definition solve_part_1 (s : string): option N := find_most_elf <$> parseInput s.
+
+Module NOrder <: TotalLeBool.
+  Definition t := N.
+  Definition leb x y := N.leb x y.
+  Print leb.
+  (* Infix "<=?" := leb (at level 70, no associativity). *)
+  Theorem leb_total : forall a1 a2, leb a1 a2 = true \/ leb a2 a1 = true.
+  Proof.
+    intros a1 a2. 
+    set (G := N.leb_spec a1 a2). 
+    inversion G.
+    - auto.
+    - set (J := N.leb_spec a2 a1).
+      inversion J.
+      * right. auto.
+      * exfalso. set (K := N.lt_asymm a1 a2 H2). auto.
   Qed.
-  
-Theorem lt_is_minus_zero : forall (a b : N), a <= b -> a - b = 0.
-Proof.
-  induction a.
-  - simpl. reflexivity.
-  - induction p.
-    + simpl. Admitted.
-  
-Theorem count_increases_same_for_same :
-  forall x y rest, y <= x -> count_increases (y :: rest) = count_increases (x :: y :: rest).
-Proof.
-  intros x y rest H.
-  unfold count_increases at 2.
-  set (G := N.leb_spec0 1%N (y - x)).
-  inversion G.
-  - fold count_increases.
-    clear G H0.
-    exfalso.
-    apply N.sub_0_le in H.
-    rewrite H in H1.
-    apply (N.nle_succ_0 0).
-    simpl. assumption.
-  - reflexivity.
-  Qed.
+End NOrder.
 
-Existing Instance Functor_option.
+Module Import NSort := Sort NOrder.
 
-Definition solve_part_1 (s : string): option N := count_increases <$> parseInput s.
+Definition sort_elves (elves : list (list N)): list N :=
+  sort (map sum_elf elves).
 
-Fixpoint group_3 (l : list N) : list N := 
-  match l with
-  | h1 :: t1 =>
-      match t1 with
-      | h2 :: t2 => 
-          match t2 with
-          | h3 :: t3 => h1 + h2 + h3 :: group_3 t1
-          | [] => []
-          end
-      | [] => []
-      end
-  | [] => []
-  end.
-  
-Theorem group_3_is_three :
-  forall x y z rest, group_3 (x :: y :: z :: rest) = (x + y + z) :: group_3 (y :: z :: rest).
-Proof.
-  intros. simpl. reflexivity.
-Qed.
-  
-Definition count_increases_in_groups (l : list N) : N := count_increases (group_3 l).
-  
-Example count_increases_in_groups_example :
-  count_increases_in_groups [199%N; 200%N; 208%N; 210%N; 200%N; 207%N; 240%N; 269%N; 260%N; 263%N] = 5.
-Proof. reflexivity. Qed.
-
-Definition solve_part_2 (s : string): option N := count_increases_in_groups <$> parseInput s.
+Definition solve_part_2 (s : string): option (list N) := sort_elves <$> parseInput s.
 
 (********************************)
 (* Extraction Language: Haskell *)
